src/Spec/ExampleH.v
@@ -1,0 +1,884 @@
+Require Import Helpers.Helpers.
+Require Import Helpers.ListStuff.
+Require Import ConcurProc.
+Require Import Equiv.
+Require Import Omega.
+Require Import FunctionalExtensionality.
+Require Import Relations.Relation_Operators.
+Require Import RelationClasses.
+Require Import Morphisms.
+Require Import List.
+Require Import Compile.
+Require Import CompileLoop.
+Require Import Modules.
+Require Import Movers.
+Require Import Abstraction.
+Require Import Protocol.
+Require Import Horizontal.
+
+
+Import ListNotations.
+
+Global Set Implicit Arguments.
+Global Generalizable All Variables.
+
+
+(** Opcodes and states *)
+
+Inductive TASOpT : Type -> Type :=
+| TestAndSet :TASOpT bool
+| Clear : TASOpT unit
+| ReadTAS : TASOpT nat
+| WriteTAS : nat -> TASOpT unit.
+
+Inductive LockOpT : Type -> Type :=
+| Acquire : LockOpT bool
+| Release : LockOpT unit
+| Read : LockOpT nat
+| Write : nat -> LockOpT unit.
+
+Inductive CounterOpT : Type -> Type :=
+| Inc : CounterOpT nat
+| Dec : CounterOpT nat.
+
+Record TASState := mkTASState {
+  TASValue : nat;
+  TASLock : bool;
+}.
+
+Record LockState := mkState {
+  Value : nat;
+  Lock : option nat;
+}.
+
+Definition CounterState := nat.
+
+
+(** Layer definitions *)
+
+Module TASAPI <: Layer.
+
+  Definition opT := TASOpT.
+  Definition State := TASState.
+
+  Inductive xstep : forall T, opT T -> nat -> State -> T -> State -> list event -> Prop :=
+  | StepTAS : forall tid v l,
+    xstep TestAndSet tid (mkTASState v l) l (mkTASState v true) nil
+  | StepClear : forall tid v l,
+    xstep Clear tid (mkTASState v l) tt (mkTASState v false) nil
+  | StepRead : forall tid v l,
+    xstep ReadTAS tid (mkTASState v l) v (mkTASState v l) nil
+  | StepWrite : forall tid v0 v l,
+    xstep (WriteTAS v) tid (mkTASState v0 l) tt (mkTASState v l) nil
+  .
+
+  Definition step := xstep.
+
+  Definition initP s :=
+    TASLock s = false.
+
+End TASAPI.
+
+
+Module TASLockAPI <: Layer.
+
+  Definition opT := TASOpT.
+  Definition State := LockState.
+
+  Inductive xstep : forall T, opT T -> nat -> State -> T -> State -> list event -> Prop :=
+  | StepTAS0 : forall tid v,
+    xstep TestAndSet tid (mkState v None) false (mkState v (Some tid)) nil
+  | StepTAS1 : forall tid tid' v,
+    xstep TestAndSet tid (mkState v (Some tid')) true (mkState v (Some tid')) nil
+  | StepClear : forall tid v l,
+    xstep Clear tid (mkState v l) tt (mkState v None) nil
+  | StepRead : forall tid v l,
+    xstep ReadTAS tid (mkState v l) v (mkState v l) nil
+  | StepWrite : forall tid v0 v l,
+    xstep (WriteTAS v) tid (mkState v0 l) tt (mkState v l) nil
+  .
+
+  Definition step := xstep.
+
+  Definition initP s :=
+    Lock s = None.
+
+End TASLockAPI.
+
+
+Module RawLockAPI <: Layer.
+
+  Definition opT := LockOpT.
+  Definition State := LockState.
+
+  Inductive xstep : forall T, opT T -> nat -> State -> T -> State -> list event -> Prop :=
+  | StepAcquire : forall tid v r,
+    xstep Acquire tid (mkState v None) r (mkState v (Some tid)) nil
+  | StepRelease : forall tid v l,
+    xstep Release tid (mkState v l) tt (mkState v None) nil
+  | StepRead : forall tid v l,
+    xstep Read tid (mkState v l) v (mkState v l) nil
+  | StepWrite : forall tid v0 v l,
+    xstep (Write v) tid (mkState v0 l) tt (mkState v l) nil
+  .
+
+  Definition step := xstep.
+
+  Definition initP s :=
+    Lock s = None.
+
+End RawLockAPI.
+
+
+Module LockAPI <: Layer.
+
+  Definition opT := LockOpT.
+  Definition State := LockState.
+
+  Inductive step_allow : forall T, opT T -> nat -> State -> Prop :=
+  | StepAcquire : forall tid s,
+    step_allow Acquire tid s
+  | StepRelease : forall tid v,
+    step_allow Release tid (mkState v (Some tid))
+  | StepRead : forall tid v,
+    step_allow Read tid (mkState v (Some tid))
+  | StepWrite : forall tid v0 v,
+    step_allow (Write v) tid (mkState v0 (Some tid)).
+
+  Definition step :=
+    nilpotent_step RawLockAPI.step step_allow.
+
+  Definition initP s :=
+    Lock s = None.
+
+End LockAPI.
+
+
+
+
+Module LockedCounterAPI <: Layer.
+
+  Definition opT := CounterOpT.
+  Definition State := LockState.
+
+  Inductive xstep : forall T, opT T -> nat -> State -> T -> State -> list event -> Prop :=
+  | StepInc : forall tid v,
+    xstep Inc tid (mkState v None) v (mkState (v + 1) None) nil
+  | StepDec : forall tid v,
+    xstep Dec tid (mkState v None) v (mkState (v - 1) None) nil.
+
+  Definition step := xstep.
+
+  Definition initP s :=
+    Lock s = None.
+
+End LockedCounterAPI.
+
+
+Module CounterAPI <: Layer.
+
+  Definition opT := CounterOpT.
+  Definition State := CounterState.
+
+  Inductive xstep : forall T, opT T -> nat -> State -> T -> State -> list event -> Prop :=
+  | StepInc : forall tid v,
+    xstep Inc tid v v (v + 1) nil
+  | StepDec : forall tid v,
+    xstep Dec tid v v (v - 1) nil.
+
+  Definition step := xstep.
+
+  Definition initP (s : State) :=
+    True.
+
+End CounterAPI.
+
+
+Module HLayer (l : Layer) <: Layer.
+
+  Definition opT := horizOpT nat l.opT.
+  Definition State := horizState nat l.State.
+  Definition step := horizStep nat l.step.
+
+  Definition indexValid (i : nat) := i = 0 \/ i = 1.
+
+  Definition initP : State -> Prop :=
+    horizInitP indexValid l.initP.
+
+End HLayer.
+
+Module LockedCounterHAPI := HLayer LockedCounterAPI.
+Module CounterHAPI := HLayer CounterAPI.
+
+
+(** Locking discipline *)
+
+Module LockingRule <: ProcRule LockAPI.
+
+  Definition follows_protocol (ts : @threads_state LockAPI.opT) :=
+    forall s,
+      follows_protocol_s RawLockAPI.step LockAPI.step_allow ts s.
+
+End LockingRule.
+
+
+
+(** Abstracting away the lock details. *)
+
+Module AbsCounter <: LayerImpl LockedCounterAPI CounterAPI.
+
+  Definition absR (s1 : LockedCounterAPI.State) (s2 : CounterAPI.State) :=
+    Lock s1 = None /\
+    Value s1 = s2.
+
+  Definition compile_ts (ts : @threads_state CounterAPI.opT) := ts.
+
+  Theorem compile_ts_no_atomics :
+    forall (ts : @threads_state CounterAPI.opT),
+      no_atomics_ts ts ->
+      no_atomics_ts (compile_ts ts).
+  Proof.
+    unfold compile_ts; eauto.
+  Qed.
+
+  Theorem absR_ok :
+    op_abs absR LockedCounterAPI.step CounterAPI.step.
+  Proof.
+    unfold op_abs; intros.
+    destruct s1; inversion H; clear H.
+    simpl in *; subst.
+    unfold absR.
+    destruct op; inversion H0; clear H0; repeat sigT_eq.
+    all: eexists; intuition eauto; constructor.
+  Qed.
+
+  Hint Resolve absR_ok.
+
+  Theorem compile_traces_match :
+    forall ts,
+      no_atomics_ts ts ->
+      traces_match_abs absR LockedCounterAPI.initP LockedCounterAPI.step CounterAPI.step (compile_ts ts) ts.
+  Proof.
+    unfold compile_ts, traces_match_abs; intros.
+    eexists; intuition idtac.
+    eapply trace_incl_abs; eauto.
+    eauto.
+  Qed.
+
+  Theorem absInitP :
+    forall s1 s2,
+      LockedCounterAPI.initP s1 ->
+      absR s1 s2 ->
+      CounterAPI.initP s2.
+  Proof.
+    firstorder.
+  Qed.
+
+End AbsCounter.
+
+
+Module AbsCounterH <: LayerImpl LockedCounterHAPI CounterHAPI.
+
+  Definition absR := horizAbsR nat AbsCounter.absR.
+
+  Definition compile_ts (ts : @threads_state CounterHAPI.opT) := ts.
+
+  Theorem compile_ts_no_atomics :
+    forall (ts : @threads_state CounterHAPI.opT),
+      no_atomics_ts ts ->
+      no_atomics_ts (compile_ts ts).
+  Proof.
+    unfold compile_ts; eauto.
+  Qed.
+
+  Theorem absR_ok :
+    op_abs absR LockedCounterHAPI.step CounterHAPI.step.
+  Proof.
+    eapply horizAbsR_ok.
+    apply AbsCounter.absR_ok.
+  Qed.
+
+  Hint Resolve absR_ok.
+
+  Theorem compile_traces_match :
+    forall ts,
+      no_atomics_ts ts ->
+      traces_match_abs absR LockedCounterHAPI.initP LockedCounterHAPI.step CounterHAPI.step (compile_ts ts) ts.
+  Proof.
+    unfold compile_ts, traces_match_abs; intros.
+    eexists; intuition idtac.
+    eapply trace_incl_abs; eauto.
+    eauto.
+  Qed.
+
+  Theorem absInitP :
+    forall s1 s2,
+      LockedCounterHAPI.initP s1 ->
+      absR s1 s2 ->
+      CounterHAPI.initP s2.
+  Proof.
+    eapply horizAbsR_initP_ok.
+    eapply AbsCounter.absInitP.
+  Qed.
+
+End AbsCounterH.
+
+
+
+(** Using locks to get atomicity. *)
+
+Module LockingCounter <: LayerImplFollowsRule LockAPI LockedCounterAPI LockingRule.
+
+  Definition inc_core : proc LockAPI.opT _ :=
+    _ <- Op Acquire;
+    v <- Op Read;
+    _ <- Op (Write (v + 1));
+    _ <- Op Release;
+    Ret v.
+
+  Definition dec_core : proc LockAPI.opT _ :=
+    _ <- Op Acquire;
+    v <- Op Read;
+    _ <- Op (Write (v - 1));
+    _ <- Op Release;
+    Ret v.
+
+  Definition compile_op T (op : LockedCounterAPI.opT T)
+                        : proc LockAPI.opT T :=
+    match op with
+    | Inc => inc_core
+    | Dec => dec_core
+    end.
+
+  Ltac step_inv :=
+    match goal with
+    | H : LockAPI.step _ _ _ _ _ _ |- _ =>
+      inversion H; clear H; subst; repeat sigT_eq
+    | H : LockAPI.step_allow _ _ _ |- _ =>
+      inversion H; clear H; subst; repeat sigT_eq
+    | H : LockAPI.step_allow _ _ _ -> False |- _ =>
+      solve [ exfalso; eauto ]
+    | H : RawLockAPI.step _ _ _ _ _ _ |- _ =>
+      inversion H; clear H; subst; repeat sigT_eq
+    | H : LockedCounterAPI.step _ _ _ _ _ _ |- _ =>
+      inversion H; clear H; subst; repeat sigT_eq
+    end; intuition idtac.
+
+  Hint Extern 1 (RawLockAPI.step _ _ _ _ _ _) => econstructor.
+  Hint Extern 1 (LockAPI.step _ _ _ _ _ _) => left.
+  Hint Extern 1 (LockAPI.step _ _ _ _ _ _) => right.
+  Hint Extern 1 (LockAPI.step_allow _ _ _) => econstructor.
+  Hint Extern 1 (LockedCounterAPI.step _ _ _ _ _ _) => econstructor.
+  Hint Extern 1 (~ LockAPI.step_allow _ _ _) => intro H'; inversion H'.
+  Hint Extern 1 (LockAPI.step_allow _ _ _ -> False) => intro H'; inversion H'.
+
+  Lemma acquire_right_mover :
+    right_mover LockAPI.step Acquire.
+  Proof.
+    unfold right_mover; intros.
+    repeat step_inv; try congruence; eauto;
+      try solve [ exfalso; eauto ].
+
+    destruct op1; repeat step_inv; eauto 10;
+      try solve [ exfalso; eauto ].
+  Qed.
+
+  Lemma release_left_mover :
+    left_mover LockAPI.step Release.
+  Proof.
+    split.
+    - eapply always_enabled_to_stable.
+      unfold always_enabled, enabled_in; intros.
+      destruct s. destruct Lock0. destruct (n == tid); subst.
+      all: eauto 10.
+    - unfold left_mover; intros.
+      repeat step_inv; try congruence; subst; eauto 10.
+      destruct op0; eauto 10.
+  Unshelve.
+    all: exact tt.
+  Qed.
+
+  Lemma read_right_mover :
+    right_mover LockAPI.step Read.
+  Proof.
+    unfold right_mover; intros.
+    repeat step_inv; try congruence; subst; eauto 10.
+  Qed.
+
+  Lemma write_right_mover : forall v,
+    right_mover LockAPI.step (Write v).
+  Proof.
+    unfold right_mover; intros.
+    repeat step_inv; try congruence; subst; eauto 10.
+    destruct op1; eauto 10.
+  Qed.
+
+  Hint Resolve acquire_right_mover.
+  Hint Resolve release_left_mover.
+  Hint Resolve read_right_mover.
+  Hint Resolve write_right_mover.
+
+
+  Theorem inc_atomic : forall `(rx : _ -> proc _ T),
+    trace_incl LockAPI.step
+      (Bind (compile_op Inc) rx)
+      (Bind (atomize compile_op Inc) rx).
+  Proof.
+    intros.
+    eapply trace_incl_atomize_ysa.
+    simpl.
+    unfold inc_core, ysa_movers; eauto 20.
+  Qed.
+
+  Theorem dec_atomic : forall `(rx : _ -> proc _ T),
+    trace_incl LockAPI.step
+      (Bind (compile_op Dec) rx)
+      (Bind (atomize compile_op Dec) rx).
+  Proof.
+    intros.
+    eapply trace_incl_atomize_ysa.
+    simpl.
+    unfold dec_core, ysa_movers; eauto 20.
+  Qed.
+
+  Theorem my_compile_correct :
+    compile_correct compile_op LockAPI.step LockedCounterAPI.step.
+  Proof.
+    unfold compile_correct; intros.
+    destruct op.
+
+    + repeat atomic_exec_inv.
+      simpl; intuition eauto.
+      repeat step_inv; eauto.
+
+    + repeat atomic_exec_inv.
+      simpl; intuition eauto.
+      repeat step_inv; eauto.
+  Qed.
+
+  Theorem my_atomize_correct :
+    atomize_correct compile_op LockAPI.step.
+  Proof.
+    unfold atomize_correct; intros.
+    destruct op.
+    + rewrite inc_atomic.
+      eapply trace_incl_bind_a.
+      eauto.
+    + rewrite dec_atomic.
+      eapply trace_incl_bind_a.
+      eauto.
+  Qed.
+
+  Hint Resolve my_compile_correct.
+  Hint Resolve my_atomize_correct.
+
+
+  Theorem all_traces_match :
+    forall ts1 ts2,
+      proc_match (Compile.compile_ok compile_op) ts1 ts2 ->
+      traces_match_ts LockAPI.step LockedCounterAPI.step ts1 ts2.
+  Proof.
+    intros.
+    eapply Compile.compile_traces_match_ts; eauto.
+  Qed.
+
+  Definition absR (s1 : LockAPI.State) (s2 : LockedCounterAPI.State) :=
+    s1 = s2.
+
+  Definition compile_ts := Compile.compile_ts compile_op.
+
+  Theorem compile_ts_no_atomics :
+    forall ts,
+      no_atomics_ts ts ->
+      no_atomics_ts (compile_ts ts).
+  Proof.
+    eapply Compile.compile_ts_no_atomics.
+    destruct op; compute; eauto.
+  Qed.
+
+  Theorem compile_traces_match :
+    forall ts2,
+      no_atomics_ts ts2 ->
+      traces_match_abs absR LockAPI.initP LockAPI.step LockedCounterAPI.step (compile_ts ts2) ts2.
+  Proof.
+    unfold traces_match_abs; intros.
+    rewrite H2 in *; clear H2.
+    eapply all_traces_match; eauto.
+    eapply Compile.compile_ts_ok; eauto.
+  Qed.
+
+
+  Theorem exec_others_preserves_lock :
+    forall tid s s',
+      exec_others (restricted_step RawLockAPI.step LockAPI.step_allow) tid s s' ->
+      Lock s = Some tid ->
+      Lock s' = Some tid.
+  Proof.
+    induction 1; intros; eauto.
+    repeat deex.
+    clear H0.
+    assert (Lock x = Lock y).
+    {
+      clear IHclos_refl_trans_1n.
+      unfold restricted_step in *; intuition idtac;
+        repeat step_inv; simpl in *; congruence.
+    }
+    rewrite IHclos_refl_trans_1n; congruence.
+  Qed.
+
+  Ltac exec_propagate :=
+    match goal with
+    | s : RawLockAPI.State |- _ =>
+      destruct s
+    | H : exec_any _ _ _ (Op _) _ _ |- _ =>
+      eapply exec_any_op in H; repeat deex
+    | H : exec_others _ _ _ _ |- _ =>
+      eapply exec_others_preserves_lock in H; simpl in *; subst; [ | congruence ]
+    end.
+
+  Lemma inc_follows_protocol : forall tid s,
+    follows_protocol_proc RawLockAPI.step LockAPI.step_allow tid s inc_core.
+  Proof.
+    intros.
+    constructor; intros.
+      constructor; intros. eauto.
+
+    repeat exec_propagate.
+      unfold restricted_step in *; intuition idtac; repeat step_inv.
+    constructor; intros.
+      constructor; intros. eauto.
+
+    repeat exec_propagate.
+      unfold restricted_step in *; intuition idtac; repeat step_inv.
+    constructor; intros.
+      constructor; intros. eauto.
+
+    repeat exec_propagate.
+      unfold restricted_step in *; intuition idtac; repeat step_inv.
+    constructor; intros.
+      constructor; intros. eauto.
+
+    repeat exec_propagate.
+      unfold restricted_step in *; intuition idtac; repeat step_inv.
+    constructor; intros.
+  Qed.
+
+  Lemma dec_follows_protocol : forall tid s,
+    follows_protocol_proc RawLockAPI.step LockAPI.step_allow tid s dec_core.
+  Proof.
+    intros.
+    constructor; intros.
+      constructor; intros. eauto.
+
+    repeat exec_propagate.
+      unfold restricted_step in *; intuition idtac; repeat step_inv.
+    constructor; intros.
+      constructor; intros. eauto.
+
+    repeat exec_propagate.
+      unfold restricted_step in *; intuition idtac; repeat step_inv.
+    constructor; intros.
+      constructor; intros. eauto.
+
+    repeat exec_propagate.
+      unfold restricted_step in *; intuition idtac; repeat step_inv.
+    constructor; intros.
+      constructor; intros. eauto.
+
+    repeat exec_propagate.
+      unfold restricted_step in *; intuition idtac; repeat step_inv.
+    constructor; intros.
+  Qed.
+
+  Hint Resolve inc_follows_protocol.
+  Hint Resolve dec_follows_protocol.
+
+  Theorem compile_ts_follows_protocol :
+    forall ts,
+      no_atomics_ts ts ->
+      LockingRule.follows_protocol (compile_ts ts).
+  Proof.
+    unfold compile_ts.
+    unfold LockingRule.follows_protocol.
+    unfold follows_protocol_s.
+    intros.
+    eapply compile_ts_follows_protocol_proc; try eassumption.
+    intros.
+
+    destruct op; simpl; eauto.
+  Qed.
+
+  Theorem absInitP :
+    forall s1 s2,
+      LockAPI.initP s1 ->
+      absR s1 s2 ->
+      LockedCounterAPI.initP s2.
+  Proof.
+    congruence.
+  Qed.
+
+End LockingCounter.
+
+
+
+
+(** Adding ghost state to the test-and-set bit. *)
+
+Module AbsLock <: LayerImpl TASAPI TASLockAPI.
+
+  Definition absR (s1 : TASAPI.State) (s2 : TASLockAPI.State) :=
+    TASValue s1 = Value s2 /\
+    (TASLock s1 = false /\ Lock s2 = None \/
+     exists tid,
+     TASLock s1 = true /\ Lock s2 = Some tid).
+
+  Definition compile_ts (ts : @threads_state TASLockAPI.opT) := ts.
+
+  Theorem compile_ts_no_atomics :
+    forall (ts : @threads_state TASLockAPI.opT),
+      no_atomics_ts ts ->
+      no_atomics_ts (compile_ts ts).
+  Proof.
+    unfold compile_ts; eauto.
+  Qed.
+
+  Hint Constructors TASLockAPI.xstep.
+
+  Theorem absR_ok :
+    op_abs absR TASAPI.step TASLockAPI.step.
+  Proof.
+    unfold op_abs; intros.
+    destruct s1; destruct s2; unfold absR in *.
+    unfold TASLockAPI.step.
+    ( intuition idtac ); simpl in *; subst; repeat deex.
+    - inversion H0; clear H0; subst; repeat sigT_eq; simpl in *.
+      all: eexists; (intuition idtac); [ | | eauto ].
+      all: simpl; eauto.
+    - inversion H0; clear H0; subst; repeat sigT_eq; simpl in *.
+      all: eexists; (intuition idtac); [ | | eauto ].
+      all: simpl; eauto.
+  Qed.
+
+  Hint Resolve absR_ok.
+
+  Theorem compile_traces_match :
+    forall ts,
+      no_atomics_ts ts ->
+      traces_match_abs absR TASAPI.initP TASAPI.step TASLockAPI.step (compile_ts ts) ts.
+  Proof.
+    unfold compile_ts, traces_match_abs; intros.
+    eexists; intuition idtac.
+    eapply trace_incl_abs; eauto.
+    eauto.
+  Qed.
+
+  Theorem absInitP :
+    forall s1 s2,
+      TASAPI.initP s1 ->
+      absR s1 s2 ->
+      TASLockAPI.initP s2.
+  Proof.
+    unfold absR, TASAPI.initP, TASLockAPI.initP.
+    intuition eauto.
+    deex; congruence.
+  Qed.
+
+End AbsLock.
+
+
+(** Implement [Acquire] on top of test-and-set *)
+
+Module LockImpl <: LayerImpl TASLockAPI RawLockAPI.
+
+  Definition acquire_cond (r : bool) :=
+    if r == false then true else false.
+
+  Definition once_cond {T} (r : T) :=
+    true.
+
+  Definition compile_op T (op : RawLockAPI.opT T) : (option T -> TASLockAPI.opT T) * (T -> bool) * option T :=
+    match op with
+    | Acquire => (fun _ => TestAndSet, acquire_cond, None)
+    | Release => (fun _ => Clear, once_cond, None)
+    | Read => (fun _ => ReadTAS, once_cond, None)
+    | Write v => (fun _ => WriteTAS v, once_cond, None)
+    end.
+
+  Definition compile_ts ts :=
+    CompileLoop.compile_ts compile_op ts.
+
+  Theorem compile_ts_no_atomics :
+    forall ts,
+      no_atomics_ts ts ->
+      no_atomics_ts (compile_ts ts).
+  Proof.
+    eapply CompileLoop.compile_ts_no_atomics.
+  Qed.
+
+  Definition absR (s1 : TASLockAPI.State) (s2 : RawLockAPI.State) :=
+    s1 = s2.
+
+  Ltac step_inv :=
+    match goal with
+    | H : TASLockAPI.step _ _ _ _ _ _ |- _ =>
+      inversion H; clear H; subst; repeat sigT_eq
+    | H : RawLockAPI.step _ _ _ _ _ _ |- _ =>
+      inversion H; clear H; subst; repeat sigT_eq
+    end.
+
+  Ltac pair_inv :=
+    match goal with
+    | H : (_, _) = (_, _) |- _ =>
+      inversion H; clear H; subst; repeat sigT_eq
+    end.
+
+  Hint Constructors RawLockAPI.xstep.
+
+  Theorem noop_or_success :
+    noop_or_success compile_op TASLockAPI.step RawLockAPI.step.
+  Proof.
+    unfold noop_or_success.
+    unfold RawLockAPI.step.
+    destruct opM; simpl; intros; pair_inv; step_inv; eauto.
+  Qed.
+
+  Theorem compile_traces_match :
+    forall ts,
+      no_atomics_ts ts ->
+      traces_match_abs absR TASLockAPI.initP TASLockAPI.step RawLockAPI.step (compile_ts ts) ts.
+  Proof.
+    unfold traces_match_abs, absR; intros; subst.
+    eapply CompileLoop.compile_traces_match_ts; eauto.
+    eapply noop_or_success.
+    eapply CompileLoop.compile_ts_ok; eauto.
+  Qed.
+
+  Theorem absInitP :
+    forall s1 s2,
+      TASLockAPI.initP s1 ->
+      absR s1 s2 ->
+      RawLockAPI.initP s2.
+  Proof.
+    congruence.
+  Qed.
+
+End LockImpl.
+
+
+(** Locking discipline *)
+
+Module LockProtocol <: LayerImplRequiresRule RawLockAPI LockAPI LockingRule.
+
+  Import LockingRule.
+
+  Definition absR (s1 : RawLockAPI.State) (s2 : LockAPI.State) :=
+    s1 = s2.
+
+  Ltac step_inv :=
+    match goal with
+    | H : RawLockAPI.step _ _ _ _ _ _ |- _ =>
+      inversion H; clear H; subst; repeat sigT_eq
+    | H : LockAPI.step_allow _ _ _ |- _ =>
+      inversion H; clear H; subst; repeat sigT_eq
+    | H : LockAPI.step _ _ _ _ _ _ |- _ =>
+      destruct H; intuition idtac
+    end.
+
+  Theorem allowed_stable :
+    forall `(op : LockAPI.opT T) `(op' : LockAPI.opT T') tid tid' s s' r evs,
+      tid <> tid' ->
+      LockAPI.step_allow op tid s ->
+      LockAPI.step op' tid' s r s' evs ->
+      LockAPI.step_allow op tid s'.
+  Proof.
+    intros.
+    destruct op; destruct op'; repeat step_inv; subst; eauto.
+    all: congruence.
+  Qed.
+
+  Definition compile_ts (ts : @threads_state LockAPI.opT) := ts.
+
+  Theorem compile_ts_no_atomics :
+    forall ts,
+      no_atomics_ts ts ->
+      no_atomics_ts (compile_ts ts).
+  Proof.
+    unfold compile_ts; eauto.
+  Qed.
+
+  Theorem compile_traces_match :
+    forall ts,
+      follows_protocol ts ->
+      no_atomics_ts ts ->
+      traces_match_abs absR RawLockAPI.initP RawLockAPI.step LockAPI.step (compile_ts ts) ts.
+  Proof.
+    unfold compile_ts, follows_protocol, absR.
+    unfold traces_match_abs; intros; subst.
+    clear H1.
+    specialize (H sm).
+    destruct H2.
+    induction H1; eauto.
+    specialize (H tid _ p) as Htid.
+    intuition idtac; repeat deex.
+
+    edestruct IHexec.
+      eapply follows_protocol_s_exec_tid_upd; eauto.
+      intros; eapply allowed_stable; eauto.
+      destruct result; eauto.
+
+    eexists; intuition idtac.
+    eapply ExecPrefixOne.
+      eauto.
+      eapply follows_protocol_preserves_exec_tid; eauto.
+      eauto.
+    eauto.
+  Qed.
+
+  Theorem absInitP :
+    forall s1 s2,
+      RawLockAPI.initP s1 ->
+      absR s1 s2 ->
+      LockAPI.initP s2.
+  Proof.
+    congruence.
+  Qed.
+
+End LockProtocol.
+
+
+(** Linking *)
+
+(* End-to-end stack:
+
+  TASAPI --------------------+---------+
+    [ AbsLock ]              |         |
+  TASLockAPI                [c1]       |
+    [ LockImpl ]             |         |
+  RawLockAPI ----------------+----+    |
+    [ LockProtocol ]         |    |   [c]
+  LockAPI                   [c2]  |    |
+    [ LockingCounter ]       |   [c3]  |
+  LockedCounterAPI ----------+    |    |
+    [ AbsCounter ]                |    |
+  CounterAPI ---------------------+----+
+ *)
+
+Module c1 := Link TASAPI TASLockAPI RawLockAPI AbsLock LockImpl.
+Module c2 := LinkWithRule RawLockAPI LockAPI LockedCounterAPI LockingRule LockProtocol LockingCounter.
+Module c3 := Link RawLockAPI LockedCounterAPI CounterAPI c2 AbsCounter.
+Module c := Link TASAPI RawLockAPI CounterAPI c1 c3.
+
+Print Assumptions c.compile_traces_match.
+
+
+Definition test_thread :=
+  Until
+    (fun _ => false)
+    (fun _ => _ <- Op Inc; _ <- Op Dec; Ret tt)
+    None.
+
+Definition test_threads :=
+  repeat (Proc test_thread) 16.
+
+Definition compiled_threads :=
+  c.compile_ts test_threads.
